general associativity lemmas for different operations

theories/prob_eff_lang/probblaze/examples/DH_KE/new_composition.v
@@ -28,15 +28,16 @@ Section new_comp_verification.
   Context {G : clutch_group (vg:=vg) (cg:=cg)}.
   Context {vgg: @val_group_generator vg}.
   Context `{!inG Σ (exclR unitO), !inG Σ dfracO,!inG Σ (dfrac_agreeR valO)}.
+  Variable xor : expr → expr → val.
 
   Definition REAL_CHAN_DHKE : val :=
-    λ: "f", ((λ: "f", F_AUTH (DH_KE "f"))%V ||ᵣ F_OAUTH) (CHAN "f").
+    λ: "f", ((λ: "f", F_AUTH (DH_KE "f"))%V ||ᵣ F_OAUTH) (CHAN xor "f").
 
   Definition REAL_CHAN_DH_REAL : val :=
-    λ: "f", ( (λ: "f", F_AUTH (C DH_real "f"))%V ||ᵣ F_OAUTH) (CHAN "f").
+    λ: "f", ( (λ: "f", F_AUTH (C DH_real "f"))%V ||ᵣ F_OAUTH) (CHAN xor "f").
 
   Definition REAL_CHAN_DH_RAND : val :=
-    λ: "f", ((λ: "f", F_AUTH (C DH_rand "f"))%V ||ᵣ F_OAUTH) (CHAN "f").
+    λ: "f", ((λ: "f", F_AUTH (C DH_rand "f"))%V ||ᵣ F_OAUTH) (CHAN xor "f").
   
    (* F_OAUTH[ F_AUTH [DH_KE [CHAN []]]] ≤ F_OAUTH[ F_AUTH [C[DH_real][CHAN []]]] *)
   (*---------------------------------------------------------------------------*)
@@ -61,25 +62,6 @@ Section new_comp_verification.
     - admit.                    (* CHAN well-typed *)
   Admitted. 
    
- (* Lemma F_OAUTH_DHKE_C_REAL' (f1 f2 : val) (L : sem_row Σ) :
-    sem_val_typed f1 f2 (∀ᵣ θₕ, (((⊤ × (sem_ty_sum 𝟙 𝟙)) -{ θₕ }-> (Option  ⊤)) × ((sem_ty_sum 𝟙 𝟙) -{ θₕ }-> (Option  ⊤))) -{ sem_row_union  θₕ L }-> 𝟙)%T -∗    
-    BREL (REAL_CHAN_DHKE f1) ≤ (REAL_CHAN_DH_REAL f2)
-     <|⊥|> {{λ v1 v2,
-                                       ∀ (leakauth1 leakauth2 keyleak1 keyleak2 : label),
-               BREL v1 ((λ: "m", do: leakauth1 (Send "m")), (λ: "m", do: leakauth1 (Recv "m")))%V (λ: "m", do: keyleak1 "m")%V ≤ v2 ((λ: "m", do: leakauth2 (Send "m")), (λ: "m", do: leakauth2 (Recv "m")))%V (λ: "m", do: keyleak2 "m")%V <| (iLblSig_to_iLblThy (envsec_row keyleak1 keyleak2 leakauth1 leakauth2 )) ++ (iLblSig_to_iLblThy L) |> {{ (λ w1 w2, 𝟙%T w1 w2)}}}}.
-  Proof.
-  Admitted.*)
-
-   (*F_OAUTH [ F_AUTH [C[DH_real][CHAN[]]]] ≤ F_OAUTH[ F_AUTH [DH_KE [CHAN []]]] *)
-  (*----------------------------------------------------------------------------*)
- (* Lemma C_REAL_DHKE_F_OAUTH (f1 f2 : val) (L : sem_row Σ) :
-    sem_val_typed f1 f2 (∀ᵣ θₕ, (((⊤ × (sem_ty_sum 𝟙 𝟙)) -{ θₕ }-> (Option  ⊤)) × ((sem_ty_sum 𝟙 𝟙) -{ θₕ }-> (Option  ⊤))) -{ sem_row_union  θₕ L }-> 𝟙)%T -∗    
-    BREL (REAL_CHAN_DH_REAL f1) ≤ (REAL_CHAN_DHKE f2)
-     <|⊥|> {{λ v1 v2,
-                                       ∀ (leakauth1 leakauth2 keyleak1 keyleak2 : label),
-               BREL v1 ((λ: "m", do: leakauth1 (Send "m")), (λ: "m", do: leakauth1 (Recv "m")))%V (λ: "m", do: keyleak1 "m")%V ≤ v2 ((λ: "m", do: leakauth2 (Send "m")), (λ: "m", do: leakauth2 (Recv "m")))%V (λ: "m", do: keyleak2 "m")%V <| (iLblSig_to_iLblThy (envsec_row keyleak1 keyleak2 leakauth1 leakauth2 )) ++ (iLblSig_to_iLblThy L) |> {{ (λ w1 w2, 𝟙%T w1 w2)}}}}.
-  Proof.
-  Admitted.*)
 
   Lemma C_REAL_DHKE_F_OAUTH :
      ⊢ sem_val_typed REAL_CHAN_DH_REAL REAL_CHAN_DHKE (∀ᵣ θ__L ,(∀ᵣ θₕ, (((⊤ × (sem_ty_sum 𝟙 𝟙)) -{ θₕ }-> 𝟙) × ((sem_ty_sum 𝟙 𝟙) -{ θₕ }-> (Option  ⊤))) 
@@ -98,74 +80,23 @@ Section new_comp_verification.
     - admit.                    (* CHAN well-typed *)
   Admitted. 
 
-  (*F_OAUTH [F_AUTH [C[DH_real][CHAN[]]]] ≤ F_OAUTH [F_AUTH [C[DH_rand][CHAN[]]]]*)
-  (*-----------------------------------------------------------------------------*)
-  (* Lemma C_REAL_DH_RAND :
-       ⊢ sem_val_typed REAL_CHAN_DH_REAL REAL_CHAN_DH_RAND (∀ᵣ θ__L ,(∀ᵣ θₕ, (((⊤ × (sem_ty_sum 𝟙 𝟙)) -{ θₕ }-> 𝟙) × ((sem_ty_sum 𝟙 𝟙) -{ θₕ }-> (Option  ⊤))) 
-                                                                      -{ sem_row_union  θₕ θ__L }-> 𝟙)
-                                                                ⊸ (∀ᵣ θ₁,∀ᵣ θ2, (((⊤ × (𝟙 + 𝟙)) -{ θ₁ }-> 𝟙) 
-                                                                                    × ((𝟙 + 𝟙) -{ θ₁ }-> Option ⊤)) 
-                                                                                    ⊸ (((⊤ × (𝟙 + 𝟙)) -{ θ2 }-> 𝟙) 
-                                                                                    × ((𝟙 + 𝟙) -{ θ2 }-> Option ⊤)) -{ sem_row_union θ₁ (sem_row_union θ2 θ__L) }-∘ 𝟙))%T.
-     Proof.
-       iApply func_comp_left.
-       - admit.
-       - admit.
-       - iIntros (θ). iApply parallel_comp_right. *)
+ 
+  Definition DHSIM_FKE_CHAN1 : val :=
+    (λ: "f", ((λ: "f", F_AUTH (DH_SIM (F_KE "f")))%V ||ᵣ F_OAUTH) (CHAN xor "f")). 
 
+  Definition DHSIM_FKE_CHAN2 : val :=
+    (λ: "f", ((λ: "f", (λ: "f", F_AUTH (DH_SIM "f"))%V (F_KE "f"))%V ||ᵣ F_OAUTH) (CHAN xor "f")). 
 
-  (*F_OAUTH [F_AUTH [C[DH_rand][CHAN[]]]] ≤ F_OAUTH [F_AUTH [C[DH_real][CHAN[]]]]*)
-  (*----------------------------------------------------------------------------*)
-  (* Lemma C_DH_RAND_REAL (f1 f2 : val) (L : sem_row Σ) :
-       sem_val_typed f1 f2 (∀ᵣ θₕ, (((⊤ × (sem_ty_sum 𝟙 𝟙)) -{ θₕ }-> (Option  ⊤)) × ((sem_ty_sum 𝟙 𝟙) -{ θₕ }-> (Option  ⊤))) -{ sem_row_union  θₕ L }-> 𝟙)%T -∗    
-       BREL (REAL_CHAN_DH_RAND f1) ≤ (REAL_CHAN_DH_REAL f2)
-        <|⊥|> {{λ v1 v2,
-                                          ∀ (leakauth1 leakauth2 keyleak1 keyleak2 : label),
-                  BREL v1 ((λ: "m", do: leakauth1 (Send "m")), (λ: "m", do: leakauth1 (Recv "m")))%V (λ: "m", do: keyleak1 "m")%V ≤ v2 ((λ: "m", do: leakauth2 (Send "m")), (λ: "m", do: leakauth2 (Recv "m")))%V (λ: "m", do: keyleak2 "m")%V <| (iLblSig_to_iLblThy (envsec_row keyleak1 keyleak2 leakauth1 leakauth2 )) ++ (iLblSig_to_iLblThy L) |> {{ (λ w1 w2, 𝟙%T w1 w2)}}}}.
-     Proof.
-     Admitted. *)
+  Definition DHSIM_FKE_CHAN3 : val :=
+    ((F_AUTH ∘f DH_SIM) ∘F (F_KE ||ᵣ F_OAUTH)%V)%V ∘f (CHAN xor).
+    (* (λ: "f", (λ: "f" "rF" "rH", (λ: "f", F_AUTH (DH_SIM "f"))%V (λ: "rG", (F_KE ||ᵣ F_OAUTH)%V "f" "rH" "rG") "rF") (CHAN xor "f")). *)
 
- (*  Definition F_AUTH_DH_KE : val :=
-       λ: "f",
-         (F_AUTH ||ₗ DH_KE) (CHAN "f").
-    
-     
-      (*F_OAUTH [F_AUTH [DH_KE [CHAN[]]]] ≤ F_AUTH [ DH_SIM [CHAN_SIM [F_CHAN[]]]]  *)
-     (*---------------------------------------------------------------------------*)
-    Lemma SEC_CHAN_DH_KE (f1 f2 : val) (L : sem_row Σ) :
-       sem_val_typed f1 f2 (∀ᵣ θₕ, (((⊤ × (sem_ty_sum 𝟙 𝟙)) -{ θₕ }-> (Option  ⊤)) × ((sem_ty_sum 𝟙 𝟙) -{ θₕ }-> (Option  ⊤))) -{ sem_row_union  θₕ L }-> 𝟙)%T -∗    
-       BREL (F_OAUTH (F_AUTH_DH_KE f1)) ≤ (F_AUTH (DH_SIM (CHAN_SIM (F_CHAN f2))))
-        <|⊥|> {{λ v1 v2,
-                                          ∀ (leakauth1 leakauth2 keyleak1 keyleak2 : label),
-                  BREL v1 ((λ: "m", do: leakauth1 (Send "m")), (λ: "m", do: leakauth1 (Recv "m")))%V (λ: "m", do: keyleak1 "m")%V ≤ v2 ((λ: "m", do: leakauth2 (Send "m")), (λ: "m", do: leakauth2 (Recv "m")))%V (λ: "m", do: keyleak2 "m")%V <| (iLblSig_to_iLblThy (envsec_row keyleak1 keyleak2 leakauth1 leakauth2 )) ++ (iLblSig_to_iLblThy L) |> {{ (λ w1 w2, 𝟙%T w1 w2)}}}}.
-     Proof.
-     Admitted.
-    
-     (*F_AUTH[ DH_SIM [CHAN_SIM [F_CHAN[]]]] ≤ F_OAUTH [F_AUTH [DH_KE [CHAN[]]]] *)
-     (*--------------------------------------------------------------------------*)
-    Lemma DH_KE_SEC_CHAN  (f1 f2 : val) (L : sem_row Σ) :
-       sem_val_typed f1 f2 (∀ᵣ θₕ, (((⊤ × (sem_ty_sum 𝟙 𝟙)) -{ θₕ }-> (Option  ⊤)) × ((sem_ty_sum 𝟙 𝟙) -{ θₕ }-> (Option  ⊤))) -{ sem_row_union  θₕ L }-> 𝟙)%T -∗    
-       BREL (F_AUTH (DH_SIM (CHAN_SIM (F_CHAN f1)))) ≤  (F_OAUTH (F_AUTH_DH_KE f1))
-        <|⊥|> {{λ v1 v2,
-                                          ∀ (leakauth1 leakauth2 keyleak1 keyleak2 : label),
-                  BREL v1 ((λ: "m", do: leakauth1 (Send "m")), (λ: "m", do: leakauth1 (Recv "m")))%V (λ: "m", do: keyleak1 "m")%V ≤ v2 ((λ: "m", do: leakauth2 (Send "m")), (λ: "m", do: leakauth2 (Recv "m")))%V (λ: "m", do: keyleak2 "m")%V <| (iLblSig_to_iLblThy (envsec_row keyleak1 keyleak2 leakauth1 leakauth2 )) ++ (iLblSig_to_iLblThy L) |> {{ (λ w1 w2, 𝟙%T w1 w2)}}}}.
-     Proof.
-     Admitted. *)
+  Definition DHSIM_FKE_CHAN4 : val :=
+    (F_AUTH ∘f DH_SIM) ∘F (R_CHAN xor).
+    (* (λ: "f" "rF" "rH", (λ: "f", F_AUTH (DH_SIM "f"))%V (λ: "rG", (λ: "f", (F_KE ||ᵣ F_OAUTH)%V (CHAN xor "f")) "f" "rH" "rG") "rF").  *)
 
-  Definition bla0 : val :=
-    (λ: "f", ((λ: "f", F_AUTH (DH_SIM (F_KE "f")))%V ||ᵣ F_OAUTH) (CHAN "f")). 
-
-  Definition bla1 : val :=
-    (λ: "f", ((λ: "f", (λ: "f", F_AUTH (DH_SIM "f"))%V (F_KE "f"))%V ||ᵣ F_OAUTH) (CHAN "f")). 
-
-  Definition bla2 : val :=
-    (λ: "f", (λ: "f" "rF" "rH", (λ: "f", F_AUTH (DH_SIM "f"))%V (λ: "rG", (F_KE ||ᵣ F_OAUTH)%V "f" "rH" "rG") "rF") (CHAN "f")).
-
-  Definition bla3 : val :=
-    (λ: "f" "rF" "rH", (λ: "f", F_AUTH (DH_SIM "f"))%V (λ: "rG", (λ: "f", (F_KE ||ᵣ F_OAUTH)%V (CHAN "f")) "f" "rH" "rG") "rF"). 
-
-  Lemma REAL_CHAN_DH_RAND_bla : 
-    ⊢ sem_val_typed REAL_CHAN_DH_RAND bla0 (∀ᵣ θ__L ,(∀ᵣ θₕ, (((⊤ × (sem_ty_sum 𝟙 𝟙)) -{ θₕ }-> 𝟙) × ((sem_ty_sum 𝟙 𝟙) -{ θₕ }-> (Option  ⊤))) 
+  Lemma REAL_CHAN_DH_RAND_DHSIM_FKE_CHAN1 : 
+    ⊢ sem_val_typed REAL_CHAN_DH_RAND DHSIM_FKE_CHAN1 (∀ᵣ θ__L ,(∀ᵣ θₕ, (((⊤ × (sem_ty_sum 𝟙 𝟙)) -{ θₕ }-> 𝟙) × ((sem_ty_sum 𝟙 𝟙) -{ θₕ }-> (Option  ⊤))) 
                                                                    -{ sem_row_union  θₕ θ__L }-> 𝟙)
                                                              ⊸ (∀ᵣ θ1,∀ᵣ θ2, (((⊤ × (𝟙 + 𝟙)) -{ θ1 }-> 𝟙) 
                                                                                  × ((𝟙 + 𝟙) -{ θ1 }-> Option ⊤)) 
@@ -181,8 +112,8 @@ Section new_comp_verification.
     - admit.
   Admitted. 
         
-  Lemma bla0_bla1 : 
-    ⊢ sem_val_typed bla0 bla1 (∀ᵣ θ__L ,(∀ᵣ θₕ, (((⊤ × (sem_ty_sum 𝟙 𝟙)) -{ θₕ }-> 𝟙) × ((sem_ty_sum 𝟙 𝟙) -{ θₕ }-> (Option  ⊤))) 
+  Lemma DHSIM_FKE_CHAN1_DHSIM_FKE_CHAN2 : 
+    ⊢ sem_val_typed  DHSIM_FKE_CHAN1 DHSIM_FKE_CHAN2 (∀ᵣ θ__L ,(∀ᵣ θₕ, (((⊤ × (sem_ty_sum 𝟙 𝟙)) -{ θₕ }-> 𝟙) × ((sem_ty_sum 𝟙 𝟙) -{ θₕ }-> (Option  ⊤))) 
                                                                    -{ sem_row_union  θₕ θ__L }-> 𝟙)
                                                              ⊸ (∀ᵣ θ1,∀ᵣ θ2, (((⊤ × (𝟙 + 𝟙)) -{ θ1 }-> 𝟙) 
                                                                                  × ((𝟙 + 𝟙) -{ θ1 }-> Option ⊤)) 
@@ -201,8 +132,8 @@ Section new_comp_verification.
     - admit.
   Admitted. 
         
-  Lemma bla1_bla2 :
-    ⊢ sem_val_typed bla1 bla2 (∀ᵣ θ__L ,(∀ᵣ θₕ, (((⊤ × (sem_ty_sum 𝟙 𝟙)) -{ θₕ }-> 𝟙) × ((sem_ty_sum 𝟙 𝟙) -{ θₕ }-> (Option  ⊤))) 
+  Lemma DHSIM_FKE_CHAN2_DHSIM_FKE_CHAN3 :
+    ⊢ sem_val_typed DHSIM_FKE_CHAN2 DHSIM_FKE_CHAN3 (∀ᵣ θ__L ,(∀ᵣ θₕ, (((⊤ × (sem_ty_sum 𝟙 𝟙)) -{ θₕ }-> 𝟙) × ((sem_ty_sum 𝟙 𝟙) -{ θₕ }-> (Option  ⊤))) 
                                                                    -{ sem_row_union  θₕ θ__L }-> 𝟙)
                                                              ⊸ (∀ᵣ θ1,∀ᵣ θ2, (((⊤ × (𝟙 + 𝟙)) -{ θ1 }-> 𝟙) 
                                                                                  × ((𝟙 + 𝟙) -{ θ1 }-> Option ⊤)) 
@@ -213,37 +144,47 @@ Section new_comp_verification.
     iApply func_comp_left.
     - admit.                    (* closed expr *)
     - admit.                    (* closed expr *)
-    - iIntros (θ). iApply func_comp_parallel_comp_assoc.
+    - iIntros (θ). iApply func_comp_parallel_comp_assoc; try done.
       + admit.
       + admit.
       + admit.
     - admit.
   Admitted.
   
-  Lemma bla2_bla3 :
-    ⊢ sem_val_typed bla2 bla3 (∀ᵣ θ__L ,(∀ᵣ θₕ, (((⊤ × (sem_ty_sum 𝟙 𝟙)) -{ θₕ }-> 𝟙) × ((sem_ty_sum 𝟙 𝟙) -{ θₕ }-> (Option  ⊤))) 
-                                              -{ sem_row_union  θₕ θ__L }-> 𝟙)
+  Lemma DHSIM_FKE_CHAN3_DHSIM_FKE_CHAN4 :
+    ⊢ sem_val_typed DHSIM_FKE_CHAN3 DHSIM_FKE_CHAN4 (∀ᵣ θ__L ,(∀ᵣ θₕ, (((⊤ × (sem_ty_sum 𝟙 𝟙)) -{ θₕ }-> 𝟙) × ((sem_ty_sum 𝟙 𝟙) -{ θₕ }-> (Option  ⊤))) 
+                                              -{ sem_row_union  θₕ θ__L }-∘ 𝟙)
                                         ⊸ (∀ᵣ θ1,∀ᵣ θ2, (((⊤ × (𝟙 + 𝟙)) -{ θ1 }-> 𝟙) 
                                                            × ((𝟙 + 𝟙) -{ θ1 }-> Option ⊤)) 
                                                           ⊸ (((⊤ × (𝟙 + 𝟙)) -{ θ2 }-> 𝟙) 
                                                                × ((𝟙 + 𝟙) -{ θ2 }-> Option ⊤)) -{ sem_row_union θ1 (sem_row_union θ2 θ__L) }-∘ 𝟙))%T.
   Proof. 
-    unfold bla2, bla3.
-    iApply functionality_comp_func_comp_assoc. (* needs to add preconditions to the lemma *)
-  Qed. 
+    iApply functionality_comp_func_comp_assoc; first done.  
+    - admit.
+    - admit.
+    - admit.
+    - admit.
+    - admit.
+Admitted. 
 
   Definition SIMSIMFCHAN : val :=
-    (λ: "f" "rF" "rH", (λ: "f", F_AUTH (DH_SIM "f"))%V (λ: "rG", (λ: "f", CHAN_SIM (F_CHAN "f"))%V "f" "rH" "rG") "rF"). 
+    (F_AUTH ∘f DH_SIM) ∘F (CHAN_SIM ∘f F_CHAN).
+    (* (λ: "f" "rF" "rH", (λ: "f", F_AUTH (DH_SIM "f"))%V (λ: "rG", (λ: "f", CHAN_SIM (F_CHAN "f"))%V "f" "rH" "rG") "rF").  *)
 
-  Lemma bla3_SIMFCHAN :
-    ⊢ sem_val_typed bla3 SIMSIMFCHAN (∀ᵣ θ__L ,(∀ᵣ θₕ, (((⊤ × (sem_ty_sum 𝟙 𝟙)) -{ θₕ }-> 𝟙) × ((sem_ty_sum 𝟙 𝟙) -{ θₕ }-> (Option  ⊤))) 
-                                              -{ sem_row_union  θₕ θ__L }-> 𝟙)
+  Lemma DHSIM_FKE_CHAN4_SIMFCHAN :
+    ⊢ sem_val_typed DHSIM_FKE_CHAN4 SIMSIMFCHAN (∀ᵣ θ__L ,(∀ᵣ θₕ, (((⊤ × (sem_ty_sum 𝟙 𝟙)) -{ θₕ }-> 𝟙) × ((sem_ty_sum 𝟙 𝟙) -{ θₕ }-> (Option  ⊤))) 
+                                              -{ sem_row_union  θₕ θ__L }-∘ 𝟙)
                                         ⊸ (∀ᵣ θ1,∀ᵣ θ2, (((⊤ × (𝟙 + 𝟙)) -{ θ1 }-> 𝟙) 
                                                            × ((𝟙 + 𝟙) -{ θ1 }-> Option ⊤)) 
                                                           ⊸ (((⊤ × (𝟙 + 𝟙)) -{ θ2 }-> 𝟙) 
                                                                × ((𝟙 + 𝟙) -{ θ2 }-> Option ⊤)) -{ sem_row_union θ1 (sem_row_union θ2 θ__L) }-∘ 𝟙))%T.
   Proof.           
-    iApply functionality_comp_cong. (* needs to add preconditions to the lemma *)
-  Qed.                       
+    iApply functionality_comp_cong. 
+    - admit.                    (* closed *)
+    - admit.                    (* closed *)
+    - admit.                    (* closed *)
+    - unshelve iApply R_I_SCHAN; done.                    (* security of secure channel  *)
+    - admit.                    (* well-typedness *)
+  Admitted. 
 
 End new_comp_verification.
