theories/prob_eff_lang/probblaze/p_composition.v
@@ -59,10 +59,21 @@ Section parallel_composition.
       "F₁" (λ: "h₁",
              "F₂" (λ: "h₂", "f" "h₂" "h₁") "r₂") "r₁".
      (* (left_composition "F₂" "F₁" "f" "r₂" "r₁").*)
-  
- Notation " F₁ ||ₗ F₂" := (left_composition F₁ F₂)%V (at level 10).
 
- Notation "F₁ ||ᵣ F₂" := (right_composition F₁ F₂)%V (at level 10).
+  Definition functionality_composition (F G : expr) : val :=
+    (λ: "f" "rH" "rF", F (λ: "rG", G "f" "rH" "rG") "rF").
+
+
+  Notation " F₁ ||ₗ F₂" := (left_composition F₁ F₂)%V (at level 10).
+
+  Notation "F₁ ||ᵣ F₂" := (right_composition F₁ F₂)%V (at level 10).
+  
+  Notation "F '∘F' G" := (functionality_composition F G) (at level 10).
+
+  Definition func_comp (F G : expr) : val :=
+    (λ: "f", F (G "f")).
+
+  Notation "F ∘f G" := (func_comp F G) (at level 10).
 
   About sem_ty_row_forall.
   About sem_ty_type_forall.
@@ -226,12 +237,45 @@ Section parallel_composition.
   
   Definition τ__F' θ τ τ' := ((∀ᵣ θ₁, τ' θ₁ -{ sem_row_union θ₁ θ}-∘ 𝟙) ⊸ (∀ᵣ θ₂, τ θ₂ -{ sem_row_union θ₂ θ }-∘ 𝟙))%T.
 
-  Lemma func_comp_parallel_comp_assoc (F G J : val) τ1 τ2 τG τ1' τ2' θ:
-    ⊢ sem_val_typed F F (τ__F τ1 τG)-∗
-    sem_val_typed G G (τ__F' θ τG τ1') -∗
-    sem_val_typed J J (τ__F τ2 τ2') -∗
-    sem_typed [] ((λ: "f", F (G "f"))||ᵣ J) (λ: "f" "rF" "rH",  F (λ: "rG", (G ||ᵣ J) "f" "rH" "rG") "rF") ⊥ ((τ__f θ τ1' τ2') ⊸ (∀ᵣ θ1, ∀ᵣ θ2, τ1 θ1 ⊸ τ2 θ2 -{ sem_row_union θ1 (sem_row_union θ2 θ) }-∘ 𝟙))%T [].
+  Lemma func_comp_parallel_comp_assoc (F J : val) (G : expr) (f x : string) τ1 τ2 τG τ1' τ2' θ :
+    (BNamed f) ≠ (BNamed x) →
+    ⊢ sem_val_typed F F (τ__F τ2 τG)-∗
+    sem_val_typed (λ: f x, G) (λ: f x, G) (τ__F' θ τG τ1') -∗
+    sem_val_typed J J (τ__F τ1 τ2') -∗
+    sem_typed [] ((F ∘f (λ: f x, G)%V) ||ᵣ J) 
+      (F ∘F ((λ: f x, G)%V ||ᵣ J)) ⊥ ((τ__f θ τ1' τ2') ⊸ (∀ᵣ θ1, ∀ᵣ θ2, τ1 θ1 ⊸ τ2 θ2 -{ sem_row_union θ1 (sem_row_union θ2 θ) }-∘ 𝟙))%T [].
   Proof.
+    iIntros (Hfx) "#HFF #HGG #HJJ !# %vs _". simpl.
+    unfold func_comp,right_composition,functionality_composition.
+    brel_pures'.
+    iModIntro; iSplit; last done.
+    iIntros (f1 f2) "Hff".
+    brel_pures'.
+    iModIntro.
+    iIntros (θ1 θ2 v1 v1') "Hτ1".
+    brel_pures'.
+    iModIntro. 
+    iIntros (v2 v2') "Hτ2".
+    brel_pures_l 3.
+    brel_pures_r.
+    brel_pures'. 
+    rewrite decide_True; last (split; done).
+    iAssert ((∀ᵣ θ₁, τG θ₁ -{ sem_row_union θ₁ θ }-∘ 𝟙)%T 
+               (λ: x, val_subst f (λ: "h₁", J (λ: "h₂", f1 "h₂" "h₁") v1) G)%V
+               (λ: "rG", (λ: "F₁" "F₂" "f" "r₂" "r₁", "F₁" (λ: "h₁", "F₂" (λ: "h₂", "f" "h₂" "h₁") "r₂") "r₁")%V (λ: f x, G)%V J f2 v1' "rG")%V) with "[Hτ1 Hff]" as "Hgg".
+    { iIntros (θG rg1 rg2) "HτG".
+      brel_pures'.
+      rewrite decide_True; last (split; done).
+      admit. }
+    iSpecialize ("HFF" with "Hgg").
+    iApply (brel_bind [_] [_] _ []); [iApply traversable_to_iThy_nil|iApply to_iThy_le_bot|].
+    assert (to_iThyIfMono OS [] = []) as <- by done.
+    iApply (brel_mono OS with "[][$HFF]"); [iApply to_iThy_le_refl|simpl].
+    iIntros (??) "Hτ".
+    iSpecialize ("Hτ" with "Hτ2").
+    rewrite !iLblSig_to_iLblThy_distr.
+    iApply (brel_introduction_mono (iLblSig_to_iLblThy θ2 ++ iLblSig_to_iLblThy θ)); last done.
+    iApply to_iThy_le_intro'; solve_submseteq.
   Admitted.
       
   Lemma func_comp_assoc (F G J : val) τ1 τ2 τ3 τ4 : 
@@ -256,23 +300,109 @@ Section parallel_composition.
     iApply (brel_wand with "HFF").
     by iIntros (??) "!# H".
   Qed. 
+
+
     
-  Lemma functionality_comp_func_comp_assoc (F G J : expr) τ1 τ2 τ1' :
-    ⊢ (* sem_typed [] F F ⊥ _ [] -∗
-       sem_typed [] G G ⊥ _ [] -∗
-       sem_typed [] J J ⊥ _ [] -∗ *)
-      sem_val_typed (λ: "f", (λ: "f" "rF" "rH", F (λ: "rG", G "f" "rH" "rG") "rF") (J "f"))
-      (λ: "f" "rF" "rH", F (λ: "rG", (λ: "f", G (J "f")) "f" "rH" "rG") "rF") (∀ᵣ θ, τ1' θ ⊸ (∀ᵣ θ1, ∀ᵣ θ2, τ1 θ1 ⊸ τ2 θ2 -{ sem_row_union θ1 (sem_row_union θ2 θ) }-∘ 𝟙))%T. 
+  Lemma functionality_comp_func_comp_assoc (F G J : expr) (f x : string) τ1 τ2 τ1' τJ τF :
+    (BNamed f) ≠ (BNamed x) →
+     is_closed_expr ∅ F →
+     is_closed_expr ∅ G →
+    ⊢ sem_typed [] F F ⊥ (∀ᵣ θ, (∀ᵣ θF, τF θF -{ sem_row_union θF θ}-∘ 𝟙) ⊸ ∀ᵣ θ1, τ1 θ1 -{ sem_row_union θ1 θ }-∘ 𝟙)%T [] -∗
+
+    sem_typed [] G G ⊥ (∀ᵣ θ, τJ θ ⊸ ∀ᵣ θ1, τ2 θ1 ⊸ ∀ᵣ θ2, τF θ2 -{ sem_row_union θ1 (sem_row_union θ2 θ)}-∘ 𝟙)%T [] -∗
+
+    sem_typed [] (λ: f x, J) (λ: f x, J) ⊥ (∀ᵣ θ, τ1' θ ⊸ τJ θ)%T [] -∗
+
+    sem_val_typed ((F ∘F G) ∘f (λ: f x, J)%V) (F ∘F (G ∘f (λ: f x, J)%V))
+      (∀ᵣ θ, (τ1' θ) ⊸ (∀ᵣ θ1, ∀ᵣ θ2, (τ1 θ1) ⊸ (τ2 θ2) -{ sem_row_union θ1 (sem_row_union θ2 θ) }-∘ 𝟙))%T. 
   Proof. 
-  Admitted. 
+    iIntros (Hfx HFclosed HGclosed) "#HFF #HGG #HJJ".
+    iIntros (θ f1 f2) "!# Hτ1'".
+    rewrite /functionality_composition /func_comp //=.
+    brel_pures'. 
+    do 2 (erewrite subst_is_closed; try done).
+    erewrite (subst_is_closed _ F); try done.
+    iModIntro.
+    iIntros (θ1 θ2 v1 v1') "Hτ1".
+    brel_pures'.
+    iModIntro.
+    iIntros (v2 v2') "Hτ2".
+    brel_pures'.
+    erewrite !(subst_is_closed _ F); try done.
+    erewrite !(subst_is_closed _ G); try done.
+    rewrite decide_True; last (split; done).
     
-  Lemma functionality_comp_cong (F G1 G2 : expr) τ1 τ2 τ1' : 
-    ⊢ (* sem_typed [] G1 G2 ⊥ (τ1' ⊸ τ2 ⊸ τ2' -{ effs }-∘ 𝟙)%T [] -∗
-         sem_typed [] F F ⊥ ((τ2' -{ effs }-∘ 𝟙) ⊸ τ1 -{ effs' }-∘ 𝟙)%T [] -∗ *)
-      sem_val_typed (λ: "f" "rF" "rH", F (λ: "rG", G1 "f" "rH" "rG") "rF") (λ: "f" "rF" "rH", F (λ: "rG", G2 "f" "rH" "rG") "rF") (∀ᵣ θ, τ1' θ ⊸ (∀ᵣ θ1, ∀ᵣ θ2, τ1 θ1 ⊸ τ2 θ2 -{ sem_row_union θ1 (sem_row_union θ2 θ) }-∘ 𝟙))%T. 
-  Admitted. 
-  
+  Admitted.
     
+  Lemma functionality_comp_cong (F G1 G2 : expr) τ1 τ2 τ1' τF :
+     is_closed_expr ∅ F →
+     is_closed_expr ∅ G1 →
+     is_closed_expr ∅ G2 →
+    ⊢ sem_typed [] G1 G2 ⊥ (∀ᵣ θ, τ1' θ ⊸ ∀ᵣ θ1, ∀ᵣ θ2, τ1 θ1 ⊸ τF θ2 -{ sem_row_union θ1 (sem_row_union θ2 θ)}-∘ 𝟙)%T [] -∗
+      sem_typed [] F F ⊥ (∀ᵣ θ, (∀ᵣ θF, τF θF -{ sem_row_union θF θ}-∘ 𝟙) ⊸ ∀ᵣ θ1, τ2 θ1 -{ sem_row_union θ1 θ }-∘ 𝟙)%T [] -∗
+      sem_val_typed (F ∘F G1) (F ∘F G2) 
+        (∀ᵣ θ, τ1' θ ⊸ (∀ᵣ θ1, ∀ᵣ θ2, τ1 θ1 ⊸ τ2 θ2 -{ sem_row_union θ1 (sem_row_union θ2 θ) }-∘ 𝟙))%T. 
+  Proof. 
+    iIntros (HFclosed HG1closed HG2closed)  "#HGG #HFF".
+    iIntros (θ f1 f2) "!# Hτ1'".
+    rewrite /functionality_composition //=.
+    brel_pures'. 
+    iModIntro.
+    iIntros (θ1 θ2 v1 v1') "Hτ1".
+    brel_pures'.
+    iModIntro.
+    iIntros (v2 v2') "Hτ2".
+    brel_pures'.
+    iAssert ([] ⊨ₑ ∅) as "#Hempty"; first done.
+    erewrite !(subst_is_closed _ F); try done.
+    erewrite !(subst_is_closed _ G1); try done.
+    erewrite !(subst_is_closed _ G2); try done.
+    iAssert ((∀ᵣ θF, τF θF -{ sem_row_union θF (sem_row_union θ1 θ) }-∘ 𝟙)%T (λ: "rG", G1 f1 v1 "rG")%V (λ: "rG", G2 f2 v1' "rG")%V) with "[Hτ1' Hτ1]" as "Hff".
+    { iIntros (θF rG1 rG2) "HτF".
+      brel_pures'.
+      erewrite !(subst_is_closed _ G1); try done.
+      erewrite !(subst_is_closed _ G2); try done.
+      unfold sem_typed. simpl. 
+      iSpecialize ("HGG" $! ∅ with "Hempty").
+      rewrite !subst_map_empty.
+      iApply (brel_bind [_;_;_] [_;_;_]); [iApply traversable_to_iThy_nil|iApply to_iThy_le_bot|].
+      assert (to_iThyIfMono OS [] = []) as <- by done.
+      iApply (brel_mono OS with "[][$HGG]"); [iApply to_iThy_le_refl|simpl].
+      iIntros (Gv1 Gv2) "(HGGv&_)".
+      iSpecialize ("HGGv" with "Hτ1'").
+      iApply (brel_bind [_;_] [_;_]); [iApply traversable_to_iThy_nil|iApply to_iThy_le_bot|].
+      assert (to_iThyIfMono OS [] = []) as <- by done.
+      iApply (brel_mono OS with "[][$HGGv]"); [iApply to_iThy_le_refl|simpl].
+      iIntros (Gfv1 Gfv2) "HGfv".
+      iSpecialize ("HGfv" with "Hτ1").
+      iApply (brel_bind [_] [_]); [iApply traversable_to_iThy_nil|iApply to_iThy_le_bot|].
+      assert (to_iThyIfMono OS [] = []) as <- by done.
+      iApply (brel_mono OS with "[][$HGfv]"); [iApply to_iThy_le_refl|simpl].
+      iIntros (GfrGv1 GfrGv2) "HGfrGv".
+      iSpecialize ("HGfrGv" with "HτF").
+      iApply (brel_wand with "[HGfrGv]").
+      { rewrite !iLblSig_to_iLblThy_distr.
+        iApply (brel_introduction_mono ((iLblSig_to_iLblThy θ1 ++ iLblSig_to_iLblThy θF ++ iLblSig_to_iLblThy θ))).
+        { iApply to_iThy_le_intro'; solve_submseteq. }
+        done. }
+      iIntros (??) "!# $". }
+    iSpecialize ("HFF" with "Hempty").
+    rewrite !subst_map_empty.
+    iApply (brel_bind [_;_] [_;_]); [iApply traversable_to_iThy_nil|iApply to_iThy_le_bot|].
+    assert (to_iThyIfMono OS [] = []) as <- by done.
+    iApply (brel_mono OS with "[][$HFF]"); [iApply to_iThy_le_refl|simpl].
+    iIntros (Fv1 Fv2) "(HFv&_)".
+    iSpecialize ("HFv" with "Hff").
+    iApply (brel_bind [_] [_]); [iApply traversable_to_iThy_nil|iApply to_iThy_le_bot|].
+    assert (to_iThyIfMono OS [] = []) as <- by done.
+    iApply (brel_mono OS with "[][$HFv]"); [iApply to_iThy_le_refl|simpl].
+    iIntros (HFfv1 HFfv2) "HFfv".
+    iSpecialize ("HFfv" with "Hτ2").
+    rewrite !iLblSig_to_iLblThy_distr.
+    iApply (brel_introduction_mono ((iLblSig_to_iLblThy θ2 ++ iLblSig_to_iLblThy θ1 ++ iLblSig_to_iLblThy θ))).
+    { iApply to_iThy_le_intro'; solve_submseteq. }
+    iApply "HFfv".
+  Qed.
 
 End parallel_composition.
 
@@ -280,3 +410,6 @@ Notation " F₁ ||ₗ F₂" := (left_composition F₁ F₂) (at level 10).
 
 Notation "F₁ ||ᵣ F₂" := (right_composition F₁ F₂) (at level 10).
 
+Notation "F '∘F' G" := (functionality_composition F G) (at level 10). 
+
+Notation "F ∘f G" := (func_comp F G) (at level 10).
